Snapshot

providers/test/extract/temp.h
@@ -1,0 +1,3 @@
+/* Needs support from KreMLin for @CAbstract */
+struct EverCrypt_Hash_state_s_____s;
+typedef struct EverCrypt_Hash_state_s_____s EverCrypt_Hash_state_s____;
