providers/evercrypt/fst/EverCrypt.ValeGlue.fst
@@ -1,7 +1,6 @@
 (** Wrappers around Vale functions *)
 module EverCrypt.ValeGlue
 
-open EverCrypt.Helpers
 open C.Failure
 open C.Endianness
 
@@ -9,23 +8,37 @@ module U32 = FStar.UInt32
 
 ///  SHA256
 
+module T = LowStar.ToFStarBuffer
+
 /// Incremental API
 let sha256_init state =
-  Vale.Hash.SHA2_256.init state
+  let state = T.new_to_old_st state in
+  Vale.Hash.SHA2_256.init state;
+  admit ()
 
 let sha256_update state data =
-  Vale.Hash.SHA2_256.update state data
+  let state = T.new_to_old_st state in
+  let data = T.new_to_old_st data in
+  Vale.Hash.SHA2_256.update state data;
+  admit ()
 
 let sha256_update_multi state data n =
   admit();
+  let state = T.new_to_old_st state in
+  let data = T.new_to_old_st data in
   C.Loops.for 0ul n (fun _ _ -> True) (fun i ->
     let b = Buffer.offset data U32.(i *^ 64ul) in
     Vale.Hash.SHA2_256.update state b)
 
 let sha256_update_last state data n =
-  Vale.Hash.SHA2_256.update_last state data n
+  let state = T.new_to_old_st state in
+  let data = T.new_to_old_st data in
+  Vale.Hash.SHA2_256.update_last state data n;
+  admit ()
 
 let sha256_finish state hash =
+  let state = T.new_to_old_st state in
+  let hash = T.new_to_old_st hash in
   Vale.Hash.SHA2_256.finish state hash;
   // Reverse byte-order in little-endian hosts
   admit();
@@ -35,4 +48,5 @@ let sha256_finish state hash =
 
 /// All-in one
 let sha256_hash state data len =
-  failwith !$"TODO: sha256_hash/Vale"
+  failwith !$"TODO: sha256_hash/Vale";
+  admit ()
